backends/lean/Aeneas/Std/Scalar/OverflowingOps/Add.lean
@@ -1,0 +1,121 @@
+import Aeneas.Std.Scalar.Core
+import Aeneas.Std.Scalar.Elab
+
+namespace Aeneas.Std
+
+open ScalarElab
+
+/-!
+## Overflowing Addition
+-/
+
+def UScalar.overflowing_add {ty} (x y : UScalar ty) : UScalar ty × Bool :=
+  (⟨ BitVec.ofNat _ (x.val + y.val) ⟩, 2^ty.numBits ≤ x.val + y.val)
+
+def IScalar.overflowing_add {ty} (x y : IScalar ty) : IScalar ty × Bool :=
+  (⟨ BitVec.ofInt _ (x.val + y.val) ⟩,
+     ¬ (-2^(ty.numBits -1) ≤ x.val + y.val ∧ x.val + y.val < 2^(ty.numBits-1)))
+
+/- [core::num::{u8}::overflowing_add] -/
+uscalar def core.num.«%S».overflowing_add := @UScalar.overflowing_add .«%S»
+
+/- [core::num::{i8}::overflowing_add] -/
+iscalar def core.num.«%S».overflowing_add := @IScalar.overflowing_add .«%S»
+
+attribute [-simp] Bool.exists_bool
+
+theorem UScalar.overflowing_add_eq {ty} (x y : UScalar ty) :
+  let z := overflowing_add x y
+  if x.val + y.val > UScalar.max ty then
+    z.fst.val + UScalar.size ty = x.val + y.val ∧
+    z.snd = true
+  else
+    z.fst.val = x.val + y.val ∧
+    z.snd = false
+  := by
+  simp [overflowing_add]
+  simp only [val, BitVec.toNat_ofNat, max]
+  split <;> rename_i hLt
+  . split_conjs
+    . have : (x.bv.toNat + y.bv.toNat) % 2^ty.numBits =
+             (x.bv.toNat + y.bv.toNat - 2^ty.numBits) % 2^ty.numBits := by
+        rw [Nat.mod_eq_sub_mod]
+        omega
+      rw [this]; clear this
+
+      have := @Nat.mod_eq_of_lt (x.bv.toNat + y.bv.toNat - 2^ty.numBits) (2^ty.numBits) (by omega)
+      rw [this]; clear this
+      simp [size]
+      scalar_tac
+    . omega
+  . split_conjs
+    . apply Nat.mod_eq_of_lt
+      omega
+    . omega
+
+uscalar @[step_pure overflowing_add x y]
+theorem core.num.«%S».overflowing_add_eq (x y : «%S») :
+  let z := overflowing_add x y
+  if x.val + y.val > UScalar.max .«%S» then z.fst.val + UScalar.size .«%S» = x.val + y.val ∧ z.snd = true
+  else z.fst.val = x.val + y.val ∧ z.snd = false
+  := UScalar.overflowing_add_eq x y
+
+
+theorem UScalar.overflowing_add_comm {ty} (x y : UScalar ty) :
+  overflowing_add x y = overflowing_add y x := by
+  simp[overflowing_add, Nat.add_comm]
+
+theorem IScalar.overflowing_add_comm {ty} (x y : IScalar ty) :
+  overflowing_add x y = overflowing_add y x := by
+  simp[IScalar.overflowing_add, Int.add_comm]
+
+uscalar
+theorem core.num.«%S».overflowing_add_comm(x y : «%S») :
+  overflowing_add x y = overflowing_add y x := UScalar.overflowing_add_comm x y
+
+iscalar
+theorem core.num.«%S».overflowing_add_comm(x y : «%S») :
+  overflowing_add x y = overflowing_add y x := IScalar.overflowing_add_comm x y
+
+theorem UScalar.overflowing_add_assoc {ty} (x y  z : UScalar ty) :
+  (overflowing_add (overflowing_add x y).1 z).1 = (overflowing_add x (overflowing_add y z).1).1 := by
+  simp [overflowing_add]
+  simp [@BitVec.ofNat_add, BitVec.add_assoc]
+
+theorem IScalar.overflowing_add_assoc {ty} (x y  z : IScalar ty) :
+  (overflowing_add (overflowing_add x y).1 z).1 = (overflowing_add x (overflowing_add y z).1).1 := by
+  simp [overflowing_add]
+  simp [@BitVec.ofInt_add, BitVec.add_assoc]
+
+uscalar
+theorem core.num.«%S».overflowing_add_assoc(x y z : «%S») :
+  (overflowing_add (overflowing_add x y).1 z).1 = (overflowing_add x (overflowing_add y z).1).1 :=
+  UScalar.overflowing_add_assoc x y z
+
+iscalar
+theorem core.num.«%S».overflowing_add_assoc(x y z : «%S») :
+  (overflowing_add (overflowing_add x y).1 z).1 = (overflowing_add x (overflowing_add y z).1).1 :=
+  IScalar.overflowing_add_assoc x y z
+
+
+@[simp]
+theorem UScalar.overflowing_add_zero {ty} (x: UScalar ty) :
+  (overflowing_add x UScalar.zero) = (x, false) := by
+  simp [overflowing_add, UScalar.zero, hmax]
+
+@[simp]
+theorem IScalar.overflowing_add_zero {ty} (x : IScalar ty) :
+  (overflowing_add x IScalar.zero) = (x, false) := by
+  simp [overflowing_add, hmax, hmin]
+
+uscalar @[simp]
+theorem core.num.«%S».overflowing_add_zero(x : «%S») :
+  (overflowing_add x UScalar.zero) = (x, false) :=
+  UScalar.overflowing_add_zero x
+
+iscalar @[simp]
+theorem core.num.«%S».overflowing_add_zero(x : «%S») :
+  (overflowing_add x IScalar.zero) = (x, false) :=
+   IScalar.overflowing_add_zero x
+
+end Aeneas.Std
